Extract term API to OCaml

term/extract/TermImports.ml
@@ -1,0 +1,10 @@
+open CoqAPI
+open CoqAPI.BigInt
+open CoqAPI.Ctr
+open Nat0
+(* open BinInt *)
+(* open BinNums *)
+(* open CoqCtr *)
+(* open Datatypes *)
+(* open List
+open Nat *)
