term/extract/term.mli
@@ -1,0 +1,32 @@
+open CoqAPI
+
+type var
+type tm_bound
+
+type intop = | Add | Mult
+
+type tm = private
+| Tconst of BigInt.t
+| Tvar of var
+| Top of intop * tm * tm
+| Tlet of tm * tm_bound
+
+(*Type safe API*)
+val create_var : string -> var
+val t_open_bound: tm_bound -> (var * tm)
+val t_close_bound: var -> tm -> tm_bound
+
+val t_const : BigInt.t -> tm
+val t_var : var -> tm
+val t_add : tm -> tm -> tm
+val t_mult : tm -> tm -> tm
+val t_let : tm -> tm_bound -> tm
+
+val tm_traverse : (BigInt.t -> 'a) -> (var -> 'a) ->
+    (intop -> tm -> tm -> 'a -> 'a -> 'a) ->
+    (tm -> tm_bound -> 'a -> 'a -> 'a) ->
+    tm -> 'a
+
+
+(*sub_t v t1 t2 is t2[t1/v]*)
+val sub_t : var -> tm -> tm -> tm
