term/src/TermAPI.v
@@ -1,6 +1,6 @@
 Require Import Coq.Strings.String.
-Require Import Coq.ZArith.BinInt.
-Require Import Coq.Lists.List.
+Require Export Coq.ZArith.BinInt.
+Require Export Coq.Lists.List.
 Require Import Coq.Bool.Bool.
 Import ListNotations.
 Local Open Scope Z_scope.
@@ -41,7 +41,7 @@ Unset Elimination Schemes.
 Variant intop := | Add | Mult.
 
 Inductive tm := 
-| Tconst: Z -> tm
+| Tconst: CoqBigInt.t -> tm
 | Tvar: var -> tm
 | Top: intop -> tm -> tm -> tm
 | Tlet: tm -> (var * tm) -> tm.
@@ -105,63 +105,6 @@ Fixpoint fmla_ind (f: fmla) : P f :=
 
 End FmlaInd.
 
-(*Semantics*)
-
-(*Variable valuation*)
-Definition val := var -> Z.
-Definition add_val (x: var) (z: Z) (v: val) : val :=
-  fun y => if var_dec x y then z else v y.
-
-Lemma add_val_twice (x : var) (z1 z2: Z) (v: val):
-forall p,
-  add_val x z1 (add_val x z2 v) p = add_val x z1 v p.
-Proof.
-  intros p. unfold add_val. destruct (var_dec x p); subst; auto.
-Qed.
-
-Lemma add_val_switch (x y : var) (z1 z2: Z) (v: val):
-  x <> y ->
-  forall p,
-  add_val x z1 (add_val y z2 v) p = add_val y z2 (add_val x z1 v) p.
-Proof.
-  intros Hxy p. unfold add_val.
-  destruct (var_dec x p); subst; auto.
-  destruct (var_dec y p); subst; auto.
-  contradiction.
-Qed.
-
-Definition intop_rep (o: intop) : Z -> Z -> Z :=
-  match o with
-  | Add => Z.add
-  | Mult => Z.mul
-  end.
-
-Fixpoint tm_rep (v: val) (t: tm) : Z :=
-  match t with
-  | Tvar x => v x
-  | Top o t1 t2 => intop_rep o (tm_rep v t1) (tm_rep v t2)
-  | Tconst c => c
-  | Tlet t1 (x, t2) => tm_rep (add_val x (tm_rep v t1) v) t2
-  end.
-
-Definition binop_rep (b: binop) : Prop -> Prop -> Prop :=
-  match b with
-  | And => and
-  | Or => or
-  | Implies => fun x y => x -> y
-  | Iff => fun x y => x <-> y
-  end.
-
-Fixpoint fmla_rep (v: val) (f: fmla) : Prop :=
-  match f with
-  | Feq t1 t2 => (tm_rep v t1) = (tm_rep v t2)
-  | Flt t1 t2 => (tm_rep v t1) < (tm_rep v t2)
-  | Fbinop b f1 f2 => binop_rep b (fmla_rep v f1) (fmla_rep v f2)
-  | Fnot f => ~ (fmla_rep v f)
-  | Fforall (x, f) => forall d, fmla_rep (add_val x d v) f
-  | Fexists (x, f) => exists d, fmla_rep (add_val x d v) f
-  end.
-
 (*Safe binding traversal*)
 
 (*First, unsafe substitutiuon*)
@@ -183,41 +126,6 @@ Fixpoint fmla_subst_unsafe (v: var) (t: tm) (f: fmla) : fmla :=
     Fforall (x, if var_dec v x then f else fmla_subst_unsafe v t f)
   | Fexists (x, f) => 
     Fexists (x, if var_dec v x then f else fmla_subst_unsafe v t f)
-  end.
-
-(*Free variables*)
-Fixpoint tm_fv (t: tm) : list var :=
-  match t with
-  | Tvar x => [x]
-  | Tconst _ => nil
-  | Top _ t1 t2 => tm_fv t1 ++ tm_fv t2
-  | Tlet t1 (x, t2) => tm_fv t1 ++ (remove var_dec x (tm_fv t2))
-  end.
-Fixpoint fmla_fv (f: fmla) : list var :=
-  match f with
-  | Feq t1 t2 => tm_fv t1 ++ tm_fv t2
-  | Flt t1 t2 => tm_fv t1 ++ tm_fv t2
-  | Fbinop _ f1 f2 => fmla_fv f1 ++ fmla_fv f2
-  | Fnot f => fmla_fv f
-  | Fforall (x, f) => remove var_dec x (fmla_fv f)
-  | Fexists (x, f) => remove var_dec x (fmla_fv f)
-  end.
-
-(*Bound variables*)
-Fixpoint tm_bnd (t: tm) : list var :=
-  match t with
-  | Tlet t1 (x, t2) => x :: (tm_bnd t1) ++ (tm_bnd t2)
-  | Top _ t1 t2 => tm_bnd t1 ++ tm_bnd t2
-  | _ => nil
-  end.
-Fixpoint fmla_bnd (f: fmla) : list var :=
-  match f with
-  | Feq t1 t2 => tm_bnd t1 ++ tm_bnd t2
-  | Flt t1 t2 => tm_bnd t1 ++ tm_bnd t2
-  | Fbinop _ f1 f2 => fmla_bnd f1 ++ fmla_bnd f2
-  | Fnot f => fmla_bnd f
-  | Fforall (x, f) => x :: fmla_bnd f
-  | Fexists (x, f) => x :: fmla_bnd f
   end.
 
 (*Bindings and Variables*)
@@ -300,12 +208,12 @@ Local Obligation Tactic := simpl; try lia.
 (*For OCaml purposes, NOT dependently typed (but it would be
   easy to write an identical dependently typed version)*)
 Variable (T: Type).
-Variable (const_case: forall (c: Z), ctr T)
+Variable (const_case: forall (c: CoqBigInt.t), ctr T)
   (var_case: forall (x: var), ctr T)
   (op_case: forall (o: intop) (t1 t2: tm) (r1 r2: T), ctr T)
   (mult_case: forall (t1 t2: tm) (r1 r2: T), ctr T)
   (*NOTE: recursive case 2 on [t_open_bound] - b is the NEW variable*)
-  (let_case: forall (t1: tm) (x: var) (t2: tm) (r1 r2: T), ctr T).
+  (let_case: forall (t1: tm) (b: tm_bound) (r1 r2: T), ctr T).
 
 Equations tm_traverse (tm1: tm) : ctr T by wf (tm_size tm1) lt :=
   tm_traverse (Tconst c) := const_case c;
@@ -320,7 +228,7 @@ Equations tm_traverse (tm1: tm) : ctr T by wf (tm_size tm1) lt :=
     st_bind_dep _ _ _ (t_open_bound b)
       (fun y s Heq => 
         v2 <- (tm_traverse (snd y)) ;;
-        let_case t1 (fst y) (snd b) v1 v2).
+        let_case t1 ((fst y), (snd b)) v1 v2).
 Next Obligation.
 intros t1 [v1 t2] _ _ y s Hy; subst.
 simpl.
@@ -339,7 +247,7 @@ Lemma tm_traverse_let (tm1: tm) (b: tm_bound) :
     v1 <- tm_traverse tm1 ;;
     x <- t_open_bound b ;;
     v2 <- tm_traverse (snd x) ;;
-    let_case tm1 (fst x) (snd b) v1 v2.
+    let_case tm1 ((fst x), (snd b)) v1 v2.
 Proof.
   simp tm_traverse. f_equal.
   apply functional_extensionality.
@@ -358,4 +266,4 @@ Definition sub_t  (v: var) (t: tm) (tm1: tm) : ctr tm :=
     (fun c => st_ret (Tconst c))
     (fun x => st_ret (if var_dec v x then t else (Tvar x)))
     (fun o t1 t2 r1 r2 =>  st_ret (Top o r1 r2))
-    (fun t1 x t2 r1 r2 => st_ret (Tlet r1 (x, r2))) tm1.
+    (fun t1 b1 r1 r2 => st_ret (Tlet r1 (fst b1, r2))) tm1.
