term/extract/TermAPIExtract.v
@@ -1,0 +1,5 @@
+From Coq Require Import Extraction.
+From CoqCompat Require Import ExtractUtil.
+From TermAPI Require Import TermAPI.
+
+Separate Extraction TermAPI.
