term/src/SubstitutionProof.v
@@ -1,4 +1,4 @@
-From TermAPI Require Import TermAPI.
+From TermAPI Require Import TermAPI TermSemantics.
 From CoqCompat Require Export StateHoare.
 Require Import Coq.ZArith.BinInt.
 Require Import Lia.
