term/src/TermSemantics.v
@@ -1,0 +1,96 @@
+From TermAPI Require Import TermAPI.
+Local Open Scope Z_scope.
+Import ListNotations.
+
+
+(*Free variables*)
+Fixpoint tm_fv (t: tm) : list var :=
+  match t with
+  | Tvar x => [x]
+  | Tconst _ => nil
+  | Top _ t1 t2 => tm_fv t1 ++ tm_fv t2
+  | Tlet t1 (x, t2) => tm_fv t1 ++ (remove var_dec x (tm_fv t2))
+  end.
+Fixpoint fmla_fv (f: fmla) : list var :=
+  match f with
+  | Feq t1 t2 => tm_fv t1 ++ tm_fv t2
+  | Flt t1 t2 => tm_fv t1 ++ tm_fv t2
+  | Fbinop _ f1 f2 => fmla_fv f1 ++ fmla_fv f2
+  | Fnot f => fmla_fv f
+  | Fforall (x, f) => remove var_dec x (fmla_fv f)
+  | Fexists (x, f) => remove var_dec x (fmla_fv f)
+  end.
+
+(*Bound variables*)
+Fixpoint tm_bnd (t: tm) : list var :=
+  match t with
+  | Tlet t1 (x, t2) => x :: (tm_bnd t1) ++ (tm_bnd t2)
+  | Top _ t1 t2 => tm_bnd t1 ++ tm_bnd t2
+  | _ => nil
+  end.
+Fixpoint fmla_bnd (f: fmla) : list var :=
+  match f with
+  | Feq t1 t2 => tm_bnd t1 ++ tm_bnd t2
+  | Flt t1 t2 => tm_bnd t1 ++ tm_bnd t2
+  | Fbinop _ f1 f2 => fmla_bnd f1 ++ fmla_bnd f2
+  | Fnot f => fmla_bnd f
+  | Fforall (x, f) => x :: fmla_bnd f
+  | Fexists (x, f) => x :: fmla_bnd f
+  end.
+
+(*Semantics*)
+
+(*Variable valuation*)
+Definition val := var -> Z.
+Definition add_val (x: var) (z: Z) (v: val) : val :=
+  fun y => if var_dec x y then z else v y.
+
+Lemma add_val_twice (x : var) (z1 z2: Z) (v: val):
+forall p,
+  add_val x z1 (add_val x z2 v) p = add_val x z1 v p.
+Proof.
+  intros p. unfold add_val. destruct (var_dec x p); subst; auto.
+Qed.
+
+Lemma add_val_switch (x y : var) (z1 z2: Z) (v: val):
+  x <> y ->
+  forall p,
+  add_val x z1 (add_val y z2 v) p = add_val y z2 (add_val x z1 v) p.
+Proof.
+  intros Hxy p. unfold add_val.
+  destruct (var_dec x p); subst; auto.
+  destruct (var_dec y p); subst; auto.
+  contradiction.
+Qed.
+
+Definition intop_rep (o: intop) : Z -> Z -> Z :=
+  match o with
+  | Add => Z.add
+  | Mult => Z.mul
+  end.
+
+Fixpoint tm_rep (v: val) (t: tm) : Z :=
+  match t with
+  | Tvar x => v x
+  | Top o t1 t2 => intop_rep o (tm_rep v t1) (tm_rep v t2)
+  | Tconst c => c
+  | Tlet t1 (x, t2) => tm_rep (add_val x (tm_rep v t1) v) t2
+  end.
+
+Definition binop_rep (b: binop) : Prop -> Prop -> Prop :=
+  match b with
+  | And => and
+  | Or => or
+  | Implies => fun x y => x -> y
+  | Iff => fun x y => x <-> y
+  end.
+
+Fixpoint fmla_rep (v: val) (f: fmla) : Prop :=
+  match f with
+  | Feq t1 t2 => (tm_rep v t1) = (tm_rep v t2)
+  | Flt t1 t2 => (tm_rep v t1) < (tm_rep v t2)
+  | Fbinop b f1 f2 => binop_rep b (fmla_rep v f1) (fmla_rep v f2)
+  | Fnot f => ~ (fmla_rep v f)
+  | Fforall (x, f) => forall d, fmla_rep (add_val x d v) f
+  | Fexists (x, f) => exists d, fmla_rep (add_val x d v) f
+  end.
